proof/correctproof/correct_eval_pc.v
@@ -1,19 +1,18 @@
-From dx.tests Require Import DxIntegers DxValues DxMemRegion DxState DxMonad DxInstructions.
-From Coq Require Import List Lia.
+From bpf.src Require Import DxIntegers DxValues DxMonad DxMemRegion DxState DxMonad DxInstructions.
+From Coq Require Import List Lia ZArith.
 From compcert Require Import Integers Values Clight Memory.
 Import ListNotations.
-Require Import ZArith.
 
-From bpf.proof Require Import Clightlogic MatchState CorrectRel CommonLemma interpreter.
+From bpf.proof Require Import Clightlogic MatchState CorrectRel CommonLemma.
+
+From bpf.clight Require Import interpreter.
+
 
 (**
-static unsigned long long eval_pc (struct bpf_state* st) {
-  return ( *st).state_pc;
-}
-
-
-Definition eval_pc: M int64_t := fun st => Some (eval_pc st, st).
- *)
+Check eval_pc.
+eval_pc
+     : M sint32_t
+*)
 
 Section Eval_pc.
 
@@ -23,7 +22,7 @@ Section Eval_pc.
   (* [Args,Res] provides the mapping between the Coq and the C types *)
   (* Definition Args : list CompilableType := [stateCompilableType].*)
   Definition args : list Type := [].
-  Definition res : Type := (int64_t:Type).
+  Definition res : Type := (sint32_t:Type).
 
   (* [f] is a Coq Monadic function with the right type *)
   Definition f : arrow_type args (M res) := DxMonad.eval_pc.
@@ -43,11 +42,11 @@ Section Eval_pc.
     DList.DCons stateM_correct (DList.DNil _).
 
   (* [match_res] relates the Coq result and the C result *)
-  Definition match_res : res -> val -> stateM -> Memory.Mem.mem -> Prop := fun x v st m => int64_correct x v.
+  Definition match_res : res -> val -> stateM -> Memory.Mem.mem -> Prop := fun x v st m => sint32_correct x v.
 
-  Instance correct_function3_eval_pc : correct_function3 p args res f fn modifies false match_arg_list match_res.
+  Instance correct_function3_eval_pc : forall a, correct_function3 p args res f fn modifies false match_arg_list match_res a.
   Proof.
-    correct_function_from_body.
+    correct_function_from_body args.
     correct_body.
     repeat intro.
     unfold INV in H.
@@ -55,7 +54,7 @@ Section Eval_pc.
     destruct c as (H_st & Hst_casted).
     unfold stateM_correct in H_st.
     destruct H_st as (Hv_eq & Hst).
-    subst v.
+    subst.
 
     (** we need to get the value of pc in the memory *)
     destruct Hst; clear minj mregs mflags mperm.
@@ -66,30 +65,22 @@ Section Eval_pc.
        1. return value should be Vlong
        2. the memory is same
       *)
-    exists (Vlong (pc_loc st)), m, Events.E0.
+    exists (Vint (pc_loc st)), m, Events.E0.
 
     repeat split; unfold step2.
     - (* goal: Smallstep.star  _ _ (State _ (Ssequence ... *)
-      apply Smallstep.plus_star.
-      (** TODO: adding Sreturn  more info by Ltac2 *)
-      eapply Smallstep.plus_one; eauto.
-      econstructor; eauto.
-      do 2 econstructor; eauto.
-      simpl.
-      do 3 econstructor; eauto.
-      econstructor; eauto.
-      reflexivity.
-      reflexivity.
-      reflexivity.
+      repeat forward_star.
+
       unfold Coqlib.align; rewrite Ptrofs.add_zero.
       unfold Ptrofs.zero; simpl.
       rewrite Ptrofs.unsigned_repr.
       rewrite <- mpc; reflexivity.
-      rewrite Ptrofs_max_unsigned_eq64.
+      rewrite Ptrofs_max_unsigned_eq32.
       lia.
-      econstructor; eauto.
+      reflexivity.
     - simpl.
       constructor.
+      reflexivity.
   Qed.
 
 End Eval_pc.
