proof/correctproof/correct_check_mem_aux.v
@@ -10,6 +10,8 @@ From bpf.proof Require Import MatchState Clightlogic clight_exec CommonLemma Cor
 
 From bpf.proof.correctproof Require Import correct_is_well_chunk_bool correct_get_sub correct_get_add correct_get_block_ptr correct_get_start_addr correct_get_block_size.
 
+Open Scope Z_scope.
+
 Section Check_mem_aux2.
 
 (** The program contains our function of interest [fn] *)
@@ -120,335 +122,184 @@ Ltac correct_forward :=
 
 Lemma correct_function_check_mem_aux_correct : forall a, correct_function3 p args res f fn (nil) true match_arg match_res a.
 Proof.
-  intros. unfold args in a.
-  car_cdr.
-  correct_function_from_body.
+  correct_function_from_body args.
   correct_body.
   unfold f. unfold check_mem_aux2.
   simpl.
   (** goal: correct_body _ _ (bindM (is_well_chunk_bool ... *)
   correct_forward.
-  - reflexivity.
-  - reflexivity.
-  - reflexivity.
-  - typeclasses eauto.
-  -  {  unfold INV.
-      unfold var_inv_preserve.
-      intros.
-      unfold match_temp_env in *.
-      rewrite Forall_fold_right in *.
-      simpl in *.
-      intuition. clear - H2 H.
-      unfold match_elt in *;
-        unfold fst in *.
-      destruct (Maps.PTree.get _mr le);auto.
-      simpl in *.
-      destruct H2 ; split; auto.
-      eapply same_my_memory_match_region;eauto.
-    }
-  - reflexivity.
-  - reflexivity.
-  - reflexivity.
-  - prove_in_inv.
-  - prove_in_inv.
-  - reflexivity.
-  - reflexivity.
-  - intros.
-    change (match_temp_env INV le st m) in H.
+
+  reflexivity.
+  reflexivity.
+  reflexivity.
+  typeclasses eauto.
+
+  { unfold INV.
+    unfold var_inv_preserve.
+    intros.
+    unfold match_temp_env in *.
+    rewrite Forall_fold_right in *.
+    simpl in *.
+    intuition. clear - H2 H.
+    unfold match_elt in *;
+      unfold fst in *.
+    destruct (Maps.PTree.get _mr le);auto.
+    simpl in *.
+    destruct H2 ; split; auto.
+    eapply same_my_memory_match_region;eauto.
+  }
+
+  reflexivity.
+  reflexivity.
+  reflexivity.
+  prove_in_inv.
+  prove_in_inv.
+  reflexivity.
+  reflexivity.
+
+  intros.
+  change (match_temp_env INV le st m) in H.
+  unfold INV in H.
+  get_invariant _chunk.
+  exists (v::nil).
+  split.
+  unfold map_opt. unfold exec_expr. rewrite p0.
+  reflexivity.
+  intros. simpl.
+  tauto.
+
+  intros.
+  (** goal: correct_body _ _ (if x then ... *)
+  correct_forward.
+  (** goal: correct_body p val (bindM (get_block_ptr c) *)
+  eapply correct_statement_seq_body.
+  change_app_for_statement.
+  eapply correct_statement_call with (has_cast := false).
+  reflexivity.
+  reflexivity.
+  reflexivity.
+  typeclasses eauto.
+  { unfold INV.
+    unfold var_inv_preserve.
+    intros.
+    unfold match_temp_env in *.
+    rewrite Forall_fold_right in *.
+    simpl in *.
+    intuition. clear - H1 H.
+    unfold match_elt in *;
+      unfold fst in *.
+    destruct (Maps.PTree.get _mr le0);auto.
+    simpl in *.
+    destruct H1 ; split; auto.
+    eapply same_my_memory_match_region;eauto.
+  }
+  reflexivity.
+  reflexivity.
+  reflexivity.
+  prove_in_inv.
+  prove_in_inv.
+  reflexivity.
+  reflexivity.
+  intros.
+  {
+    intros.
+    change (match_temp_env (((_well_chunk, Clightdefs.tbool, stateless match_bool true) :: INV)) le0 st0 m0) in H.
     unfold INV in H.
-    get_invariant _chunk.
+    get_invariant _mr.
     exists (v::nil).
     split.
     unfold map_opt. unfold exec_expr. rewrite p0.
     reflexivity.
     intros. simpl.
-    tauto.
-  -
-    intros.
-    (** goal: correct_body _ _ (if x then ... *)
-    correct_forward.
-    (** goal: correct_body p val (bindM (get_block_ptr c) *)
-    eapply correct_statement_seq_body.
-    change_app_for_statement.
-    eapply correct_statement_call with (has_cast := false).
-    reflexivity.
-    reflexivity.
-    reflexivity.
-    typeclasses eauto.
-    { unfold INV.
-      unfold var_inv_preserve.
-      intros.
-      unfold match_temp_env in *.
-      rewrite Forall_fold_right in *.
-      simpl in *.
-      intuition. clear - H1 H.
-      unfold match_elt in *;
-        unfold fst in *.
-      destruct (Maps.PTree.get _mr le0);auto.
-      simpl in *.
-      destruct H1 ; split; auto.
-      eapply same_my_memory_match_region;eauto.
-    }
-    reflexivity.
-    reflexivity.
-    reflexivity.
-    prove_in_inv.
-    prove_in_inv.
-    reflexivity.
-    reflexivity.
-    intros.
-    {
-      intros.
-      change (match_temp_env (((_well_chunk, Clightdefs.tbool, stateless match_bool true) :: INV)) le0 st0 m0) in H.
-      unfold INV in H.
-      get_invariant _mr.
-      exists (v::nil).
-      split.
-      unfold map_opt. unfold exec_expr. rewrite p0.
-      reflexivity.
-      intros. simpl.
-      intuition. eauto.
-    }
-    intros.
-    (** goal: correct_body _ _ (bindM (get_start_addr c) ... *)
-    eapply correct_statement_seq_body.
-    change_app_for_statement.
-    eapply correct_statement_call with (has_cast := false).
-    reflexivity.
-    reflexivity.
-    reflexivity.
-    typeclasses eauto.
-    { unfold INV.
-      unfold var_inv_preserve.
-      intros.
-      unfold match_temp_env in *.
-      rewrite Forall_fold_right in *.
-      simpl in *.
-      intuition. clear - H3 H.
-      unfold match_elt in *;
-        unfold fst in *.
-      destruct (Maps.PTree.get _mr le1);auto.
-      simpl in *.
-      destruct H3 ; split; auto.
-      eapply same_my_memory_match_region;eauto.
-    }
-    reflexivity.
-    reflexivity.
-    reflexivity.
-    prove_in_inv.
-    prove_in_inv.
-    reflexivity.
-    reflexivity.
-    intros.
-    change (match_temp_env ((_ptr, Clightdefs.tuint, correct_get_block_ptr.match_res x)
-                              :: (_well_chunk, Clightdefs.tbool, stateless match_bool true) :: INV) le1 st1 m1) in H.
-    unfold INV in H.
-    get_invariant _mr.
-    exists (v::nil).
-    split.
-    unfold map_opt,exec_expr.
-    rewrite p0.
-    reflexivity.
-    simpl. intros.
-    intuition eauto.
-    intros.
-    (** goal: correct_body _ _ (bindM (get_block_size c) ... *)
-    eapply correct_statement_seq_body.
-    change_app_for_statement.
-    eapply correct_statement_call with (has_cast := false).
-    reflexivity.
-    reflexivity.
-    reflexivity.
-    typeclasses eauto.
-    { unfold INV.
-      unfold var_inv_preserve.
-      intros.
-      unfold match_temp_env in *.
-      rewrite Forall_fold_right in *.
-      simpl in *.
-      intuition. clear - H4 H.
-      unfold match_elt in *;
-        unfold fst in *.
-      destruct (Maps.PTree.get _mr le2); auto.
-      simpl in *.
-      destruct H4; split; auto.
-      eapply same_my_memory_match_region;eauto.
-    }
-    reflexivity.
-    reflexivity.
-    reflexivity.
-    prove_in_inv.
-    prove_in_inv.
-    reflexivity.
-    reflexivity.
-    intros.
-    change (match_temp_env ((_start, Clightdefs.tuint, correct_get_start_addr.match_res x0)
-         :: (_ptr, Clightdefs.tuint, correct_get_block_ptr.match_res x)
-         :: (_well_chunk, Clightdefs.tbool, stateless match_bool true) :: INV) le2 st2 m2) in H.
-    unfold INV in H.
-    get_invariant _mr.
-    (**  exists lval : list val, _ [Etempvar _mr3 _] = Some lval *)
-    exists (v::nil).
-    split.
-    unfold map_opt, exec_expr.
-    rewrite p0; reflexivity.
-    simpl;intros.
-    intuition eauto.
-    intros.
-    (** goal:  correct_body _ _ (bindM (get_sub c0 x0) ... *)
-    eapply correct_statement_seq_body.
-    change_app_for_statement.
-    eapply correct_statement_call with (has_cast := false).
-    reflexivity.
-    reflexivity.
-    reflexivity.
-    typeclasses eauto.
-    { unfold INV.
-      unfold var_inv_preserve.
-      intros.
-      unfold match_temp_env in *.
-      rewrite Forall_fold_right in *.
-      simpl in *.
-      intuition. clear - H5 H.
-      unfold match_elt in *;
-        unfold fst in *.
-      destruct (Maps.PTree.get _mr le3); auto.
-      simpl in *.
-      destruct H5; split; auto.
-      eapply same_my_memory_match_region;eauto.
-    }
-    reflexivity.
-    reflexivity.
-    reflexivity.
-    prove_in_inv.
-    prove_in_inv.
-    reflexivity.
-    reflexivity.
-    intros.
-    change (match_temp_env ((_size, Clightdefs.tuint, correct_get_block_size.match_res x1)
-         :: (_start, Clightdefs.tuint, correct_get_start_addr.match_res x0)
-            :: (_ptr, Clightdefs.tuint, correct_get_block_ptr.match_res x)
-               :: (_well_chunk, Clightdefs.tbool, stateless match_bool true) :: INV) le3 st3 m3) in H.
-    unfold INV in H.
-    get_invariant _addr.
-    get_invariant _start.
-    (**  exists lval : list val, _ [(Etempvar _addr0 _); (Etempvar _start _)] = Some lval *)
-    exists ([v; v0]).
-    split.
-    unfold map_opt, exec_expr.
-    rewrite p0, p1; reflexivity.
-    simpl;intros.
-    intuition; eauto. (**r we lost the evident that `correct_get_start_addr.match_res x0 v0 st3 m3` *)
-    eauto. (**r we lost one very imporant information: the input/output constraints *)
-    intros.
-    (** goal:  correct_body _ _ (bindM (get_add x2 (memory_chunk_to_valu32 c1)) ... *)
-    eapply correct_statement_seq_body.
-    change_app_for_statement.
-    eapply correct_statement_call with (has_cast := false).
-    reflexivity.
-    reflexivity.
-    reflexivity.
-    typeclasses eauto.
-    { unfold INV.
-      unfold var_inv_preserve.
-      intros.
-      unfold match_temp_env in *.
-      rewrite Forall_fold_right in *.
-      simpl in *.
-      intuition. clear - H6 H.
-      unfold match_elt in *;
-        unfold fst in *.
-      destruct (Maps.PTree.get _mr le4); auto.
-      simpl in *.
-      destruct H6; split; auto.
-      eapply same_my_memory_match_region;eauto.
-    }
-    reflexivity.
-    reflexivity.
-    reflexivity.
-    prove_in_inv.
-    prove_in_inv.
-    reflexivity.
-    reflexivity.
-    intros.
-    change (match_temp_env ((_lo_ofs, Clightdefs.tuint, correct_get_sub.match_res x2)
-       :: (_size, Clightdefs.tuint, correct_get_block_size.match_res x1)
-          :: (_start, Clightdefs.tuint, correct_get_start_addr.match_res x0)
-             :: (_ptr, Clightdefs.tuint, correct_get_block_ptr.match_res x)
-                :: (_well_chunk, Clightdefs.tbool, stateless match_bool true)
-                   :: INV) le4 st4 m4) in H.
-    unfold INV in H.
-    get_invariant _lo_ofs.
-    get_invariant _chunk.
-    unfold map_opt, exec_expr.
-    rewrite p0, p1.
-    exists ([v; v0]).
-    split.
-    unfold map_opt, exec_expr. reflexivity.
-    simpl;intros.
-    intuition eauto.
-
-    unfold stateless, valu32_correct, memory_chunk_to_valu32, well_chunk_Z.
-    unfold stateless, match_chunk, memory_chunk_to_valu32, well_chunk_Z in H2.
-    intuition eauto.
-    intros.
-    (** goal: correct_body _ _ (if then else ... *)
-    destruct (match x2 with
-    | Vint n2 => negb (Int.ltu n2 int32_0)
-    | _ => false
-    end && compu_lt_32 x3 x1).
-    destruct (compu_le_32 x2 (memory_chunk_to_valu32_upbound c1) &&
-    match val32_modu x2 (memory_chunk_to_valu32 c1) with
-    | Vint n2 => Int.eq int32_0 n2
-    | _ => false
-    end).
-    unfold list_rel_arg,app;
-  match goal with
-    |- correct_body _ _ _ _ ?B _ ?INV
-                 _ _ _ _ =>
-      let I := fresh "INV" in
-      set (I := INV) ; simpl in I;
-      let B1 := eval simpl in B in
-        change B with B1
-  end.
-    unfold correct_body.
-    intro.
-    destruct (returnM (Val.add x x2) st5); [idtac | constructor].
-    destruct p0.
-    intros.
-
-    eexists. exists m, Events.E0.
-    forward_star.
-    repeat forward_star.
-    eapply correct_statement_seq_body.
-    change_app_for_statement.
-    eapply correct_statement_call with (has_cast := false).
-    apply st5.
-
-    TODO. 
-    rewrite Hv0_eq in *.
-    simpl.
-    eexists.
-    split.
-    reflexivity.
-    simpl.
-    (**  exists lval : list val, _ [Etempvar _lo_ofs _; Ecast (Etempvar _chunk1 _) _] = Some lval *)
-    exists ([v; (Vlong (v0)]).
-    split.
-   
-    rewrite p0, p1.
-    simpl.
-    unfold Cop.sem_cast; simpl. (**r `Maps.PTree.get _chunk1 le4 = Some v0` where v0 should be Vint *)
-    unfold Int.one. (** Vlong vs vint: we could generate u64 chunk by dx *)
-    destruct c1; rewrite Int.unsigned_repr. reflexivity.
-    reflexivity.
-    simpl;intros.
-    intuition eauto.
-
-    
-  admit.
+    intuition. eauto.
+  }
   intros.
-  (** goal: correct_body _ _ (bindM (get_subl ... *)
+  (** goal: correct_body _ _ (bindM (get_start_addr c) ... *)
+  eapply correct_statement_seq_body.
+  change_app_for_statement.
+  eapply correct_statement_call with (has_cast := false).
+  reflexivity.
+  reflexivity.
+  reflexivity.
+  typeclasses eauto.
+  { unfold INV.
+    unfold var_inv_preserve.
+    intros.
+    unfold match_temp_env in *.
+    rewrite Forall_fold_right in *.
+    simpl in *.
+    intuition. clear - H3 H.
+    unfold match_elt in *;
+      unfold fst in *.
+    destruct (Maps.PTree.get _mr le1);auto.
+    simpl in *.
+    destruct H3 ; split; auto.
+    eapply same_my_memory_match_region;eauto.
+  }
+  reflexivity.
+  reflexivity.
+  reflexivity.
+  prove_in_inv.
+  prove_in_inv.
+  reflexivity.
+  reflexivity.
+  intros.
+  change (match_temp_env ((_ptr, Clightdefs.tuint, correct_get_block_ptr.match_res x)
+                            :: (_well_chunk, Clightdefs.tbool, stateless match_bool true) :: INV) le1 st1 m1) in H.
+  unfold INV in H.
+  get_invariant _mr.
+  exists (v::nil).
+  split.
+  unfold map_opt,exec_expr.
+  rewrite p0.
+  reflexivity.
+  simpl. intros.
+  intuition eauto.
+  intros.
+  (** goal: correct_body _ _ (bindM (get_block_size c) ... *)
+  eapply correct_statement_seq_body.
+  change_app_for_statement.
+  eapply correct_statement_call with (has_cast := false).
+  reflexivity.
+  reflexivity.
+  reflexivity.
+  typeclasses eauto.
+  { unfold INV.
+    unfold var_inv_preserve.
+    intros.
+    unfold match_temp_env in *.
+    rewrite Forall_fold_right in *.
+    simpl in *.
+    intuition. clear - H4 H.
+    unfold match_elt in *;
+      unfold fst in *.
+    destruct (Maps.PTree.get _mr le2); auto.
+    simpl in *.
+    destruct H4; split; auto.
+    eapply same_my_memory_match_region;eauto.
+  }
+  reflexivity.
+  reflexivity.
+  reflexivity.
+  prove_in_inv.
+  prove_in_inv.
+  reflexivity.
+  reflexivity.
+  intros.
+  change (match_temp_env ((_start, Clightdefs.tuint, correct_get_start_addr.match_res x0)
+       :: (_ptr, Clightdefs.tuint, correct_get_block_ptr.match_res x)
+       :: (_well_chunk, Clightdefs.tbool, stateless match_bool true) :: INV) le2 st2 m2) in H.
+  unfold INV in H.
+  get_invariant _mr.
+  (**  exists lval : list val, _ [Etempvar _mr3 _] = Some lval *)
+  exists (v::nil).
+  split.
+  unfold map_opt, exec_expr.
+  rewrite p0; reflexivity.
+  simpl;intros.
+  intuition eauto.
+  intros.
+  (** goal:  correct_body _ _ (bindM (get_sub c0 x0) ... *)
   eapply correct_statement_seq_body.
   change_app_for_statement.
   eapply correct_statement_call with (has_cast := false).
@@ -465,7 +316,7 @@ Proof.
     intuition. clear - H5 H.
     unfold match_elt in *;
       unfold fst in *.
-    destruct (Maps.PTree.get _mr3 le3); auto.
+    destruct (Maps.PTree.get _mr le3); auto.
     simpl in *.
     destruct H5; split; auto.
     eapply same_my_memory_match_region;eauto.
@@ -477,10 +328,24 @@ Proof.
   prove_in_inv.
   reflexivity.
   reflexivity.
-  admit.
   intros.
-  (** goal: correct_body _ _ (bindM (get_addl ... *)
-  unfold memory_chunk_to_val64.
+  change (match_temp_env ((_size, Clightdefs.tuint, correct_get_block_size.match_res x1)
+       :: (_start, Clightdefs.tuint, correct_get_start_addr.match_res x0)
+          :: (_ptr, Clightdefs.tuint, correct_get_block_ptr.match_res x)
+             :: (_well_chunk, Clightdefs.tbool, stateless match_bool true) :: INV) le3 st3 m3) in H.
+  unfold INV in H.
+  get_invariant _addr.
+  get_invariant _start.
+  (**  exists lval : list val, _ [(Etempvar _addr0 _); (Etempvar _start _)] = Some lval *)
+  exists ([v; v0]).
+  split.
+  unfold map_opt, exec_expr.
+  rewrite p0, p1; reflexivity.
+  simpl;intros.
+  intuition; eauto. (**r we lost the evident that `correct_get_start_addr.match_res x0 v0 st3 m3` *)
+  eauto. (**r we lost one very imporant information: the input/output constraints *)
+  intros.
+  (** goal:  correct_body _ _ (bindM (get_add x2 (memory_chunk_to_valu32 c1)) ... *)
   eapply correct_statement_seq_body.
   change_app_for_statement.
   eapply correct_statement_call with (has_cast := false).
@@ -497,12 +362,11 @@ Proof.
     intuition. clear - H6 H.
     unfold match_elt in *;
       unfold fst in *.
-    destruct (Maps.PTree.get _mr3 le4); auto.
+    destruct (Maps.PTree.get _mr le4); auto.
     simpl in *.
     destruct H6; split; auto.
     eapply same_my_memory_match_region;eauto.
   }
-  (** here is a casting from u32 -> u64 *)
   reflexivity.
   reflexivity.
   reflexivity.
@@ -511,100 +375,234 @@ Proof.
   reflexivity.
   reflexivity.
   intros.
-  change (match_temp_env ((_lo_ofs, Clightdefs.tulong, correct_get_subl.match_res x2)
-         :: (_size, Clightdefs.tulong,
-            correct_getMemRegion_block_size.match_res x1)
-            :: (_start, Clightdefs.tulong,
-               correct_getMemRegion_start_addr.match_res x0)
-               :: (_ptr, Clightdefs.tulong,
-                  correct_getMemRegion_block_ptr.match_res x)
-                  :: (_well_chunk, Clightdefs.tbool, stateless match_bool true)
-                     :: INV) le4 st4 m4) in H.
-  get_invariant _lo_ofs.
+  change (match_temp_env ((_lo_ofs, Clightdefs.tuint, correct_get_sub.match_res x2)
+     :: (_size, Clightdefs.tuint, correct_get_block_size.match_res x1)
+        :: (_start, Clightdefs.tuint, correct_get_start_addr.match_res x0)
+           :: (_ptr, Clightdefs.tuint, correct_get_block_ptr.match_res x)
+              :: (_well_chunk, Clightdefs.tbool, stateless match_bool true)
+                 :: INV) le4 st4 m4) in H.
   unfold INV in H.
-  get_invariant _chunk1.
-  destruct c3.
-  assert (exists v, Cop.sem_cast v0 Clightdefs.tuint Clightdefs.tulong m4 = Some v).
-  {
-    inv H1.
-    unfold Cop.sem_cast.
-    simpl.
-    eexists ; reflexivity.
-    unfold stateless,match_chunk in H0.
-    discriminate.
-  }
-  destruct H2 as (v1 & C).
-  exists (v::v1::nil).
+  get_invariant _lo_ofs.
+  get_invariant _chunk.
+  unfold map_opt, exec_expr.
+  rewrite p0, p1.
+  exists ([v; v0]).
   split.
-  unfold map_opt,exec_expr.
-  rewrite p0. rewrite p1.
-  simpl. rewrite C. reflexivity.
-  simpl.
+  unfold map_opt, exec_expr. reflexivity.
+  simpl;intros.
+  intuition eauto.
+
+  unfold stateless, valu32_correct, memory_chunk_to_valu32, well_chunk_Z.
+  unfold stateless, match_chunk, memory_chunk_to_valu32, well_chunk_Z in H2.
+  intuition eauto.
+  intros.
+  (** goal: correct_body _ _ (if then else ... *)
+
+  destruct (match x2 with
+  | Vint n2 => negb (Int.ltu n2 int32_0)
+  | _ => false
+  end && compu_lt_32 x3 x1) eqn: Hcond1.
+  destruct (compu_le_32 x2 (memory_chunk_to_valu32_upbound c1) &&
+  match val32_modu x2 (memory_chunk_to_valu32 c1) with
+  | Vint n2 => Int.eq int32_0 n2
+  | _ => false
+  end) eqn: Hcond2.
+  unfold list_rel_arg,app;
+  match goal with
+  |- correct_body _ _ _ _ ?B _ ?INV
+               _ _ _ _ =>
+    let I := fresh "INV" in
+    set (I := INV) ; simpl in I;
+    let B1 := eval simpl in B in
+      change B with B1
+  end.
+  unfold correct_body.
+  intro.
+  destruct (returnM (Val.add x x2) st5); [idtac | constructor].
+  destruct p0.
+  intros.
+
+  (**r we need the value of those vairable in the memory, they will be used later *)
+  unfold INV0,INV in H.
+  get_invariant_more _hi_ofs.
+  get_invariant_more _lo_ofs.
+  get_invariant_more _size.
+  get_invariant_more _chunk.
+  get_invariant_more _ptr.
+  unfold correct_get_add.match_res, valu32_correct in H1.
+  destruct H1 as (H1_eq & (vi1 & Hvi1_eq)).
+  unfold correct_get_sub.match_res, valu32_correct in H3.
+  destruct H3 as (H3_eq & (vi3 & Hvi3_eq)).
+  unfold correct_get_block_size.match_res, valu32_correct in H5.
+  destruct H5 as (H5_eq & (vi5 & Hvi5_eq)).
+  unfold stateless, match_chunk, memory_chunk_to_valu32 in H7.
+  unfold correct_get_block_ptr.match_res, valu32_correct in H9.
+  destruct H9 as (H10_eq & (vi10 & Hvi10_eq)).
+  subst.
+
+  eexists. exists m, Events.E0.
+  repeat split.
+  + 
+    Transparent Archi.ptr64.
+    forward_star.
+    repeat forward_star.
+    forward_star.
+    repeat forward_star.
+    unfold Cop.bool_val, Val.of_bool, Cop.sem_cmp, Cop.sem_binarith, Cop.sem_cast; simpl.
+    unfold Int.ltu.
+    fold Int.zero.
+    rewrite Int.unsigned_zero.
+    assert (Hvi3_ge: ((Int.unsigned vi3) >= 0)%Z). {
+      assert (Hhi_range: (0 <= Int.unsigned vi3 <= Int.max_unsigned)%Z).
+      apply Int.unsigned_range_2.
+      lia.
+    }
+    rewrite zlt_false; simpl.
+    rewrite Int_eq_one_zero; reflexivity.
+    assumption.
+
+    (** Smallstep.star _ _ (State _ (if negb false ... *)
+    simpl.
+    forward_star.
+    forward_star.
+    unfold Cop.sem_cast, Val.of_bool; simpl.
+    apply andb_prop in Hcond1.
+    destruct Hcond1 as (Hcond1_1 & Hcond1_2).
+    unfold compu_lt_32 in Hcond1_2.
+    rewrite Hcond1_2; simpl.
+    rewrite Int_eq_one_zero; reflexivity.
+    forward_star.
+    repeat forward_star.
+    forward_star.
+    repeat forward_star.
+    rewrite Maps.PTree.gss; reflexivity.
+    reflexivity.
+    (** Smallstep.star _ _(State _ (if negb (Int.eq Int.one Int.zero) then ... *)
+    forward_star.
+    rewrite Int_eq_one_zero.
+    unfold negb.
+    repeat forward_star.
+
+    (**r after we need the info about Hcond2, I do it here*)
+    apply andb_prop in Hcond2.
+    destruct Hcond2 as (Hcond2_1 & Hcond2_2).
+    unfold compu_le_32, memory_chunk_to_valu32_upbound in Hcond2_1.
+    rewrite Int_max_unsigned_eq64 in Hcond2_1.
+    unfold val32_modu, Val.modu, memory_chunk_to_valu32 in Hcond2_2.
+    
+    destruct (Int.eq (Int.repr (well_chunk_Z c1)) Int.zero) eqn: Heq_zero; try discriminate.
+
+    (**r we also need those info below *)
+    assert (Hneq1: _lo_ofs <> _t'8). {
+      unfold _lo_ofs, _t'8.
+      intro Hneq; inversion Hneq.
+    }
+    assert (Hneq2: _chunk <> _t'8). {
+      unfold _chunk, _t'8.
+      intro Hneq; inversion Hneq.
+    }
+
+    forward_star.
+    forward_star.
+    (**r the 1st place I need _lo_ofs & _chunk *)
+    apply Maps.PTree.gso with (x:=Vint Int.one) (m:=le5) in Hneq1.
+    rewrite Hneq1.
+    rewrite p1; reflexivity.
+    apply Maps.PTree.gso with (x:=Vint Int.one) (m:=le5) in Hneq2.
+    rewrite Hneq2.
+    rewrite p3; reflexivity.
+    reflexivity.
+    reflexivity.
+    unfold Cop.bool_val, Val.of_bool; simpl.
+
+    (**the first place I need Hcond2 *)
+    fold Int.mone.
+    unfold Int.sub; rewrite Int.unsigned_mone.
+    assert (He: Int.modulus - 1 = 4294967295). {
+      unfold Int.modulus, Int.wordsize, Wordsize_32.wordsize; reflexivity.
+    }
+    rewrite He.
+
+    assert (Hwell_chunk_unsigned: Int.unsigned (Int.repr (well_chunk_Z c1)) = well_chunk_Z c1). {
+      destruct c1; simpl; try (fold Int.zero; apply Int.unsigned_zero); try rewrite Int.unsigned_repr; try reflexivity; try rewrite Int_max_unsigned_eq64; try lia.
+    }
+    rewrite Hwell_chunk_unsigned.
+    rewrite Hcond2_1; simpl.
+    rewrite Int_eq_one_zero; unfold negb; reflexivity.
+    Search (if true then _ else _).
+    match goal with
+    | |- context[if true then ?X else ?Y] =>
+        change (if true then X else Y) with X
+    end.
+
+    forward_star.
+    forward_star.
+    (**r the 2nd place I need _lo_ofs & _chunk *)
+    apply Maps.PTree.gso with (x:=Vint Int.one) (m:=le5) in Hneq1.
+    rewrite Hneq1.
+    rewrite p1; reflexivity.
+    apply Maps.PTree.gso with (x:=Vint Int.one) (m:=le5) in Hneq2.
+    rewrite Hneq2.
+    rewrite p3; reflexivity.
+
+    unfold Cop.sem_binary_operation; simpl.
+    unfold Cop.sem_mod, Cop.sem_binarith; simpl.
+    (**r here we need to prove `modu`, i.e. (well_chunk_Z c1) <> 0, we should see the Hypothesis `Hcond2` *)
+    rewrite Heq_zero;
+    reflexivity.
+    reflexivity.
+
+    unfold Cop.bool_val, Val.of_bool; simpl.
+    unfold int32_0, Int.zero in Hcond2_2.
+    rewrite Hcond2_2.
+    reflexivity.
+
+    forward_star.
+    repeat forward_star.
+    forward_star.
+    repeat forward_star.
+    rewrite Maps.PTree.gss.
+    rewrite Int_eq_one_zero.
+    reflexivity.
+    reflexivity.
+
+    rewrite Int_eq_one_zero; unfold negb.
+    forward_star.
+    repeat forward_star.
+    assert (Hneq3: _ptr <> _t'7). {
+      unfold _ptr, _t'7.
+      intro Hneq; inversion Hneq.
+    }
+    assert (Hneq4: _ptr <> _t'8). {
+      unfold _ptr, _t'8.
+      intro Hneq; inversion Hneq.
+    }
+    apply Maps.PTree.gso with (x:=Vint Int.one) (m:=(Maps.PTree.set _t'8 (Vint Int.one) le5)) in Hneq3; rewrite Hneq3.
+    apply Maps.PTree.gso with (x:=Vint Int.one) (m:=le5) in Hneq4; rewrite Hneq4.
+    rewrite p4; reflexivity.
+    assert (Hneq3: _lo_ofs <> _t'7). {
+      unfold _lo_ofs, _t'7.
+      intro Hneq; inversion Hneq.
+    }
+    apply Maps.PTree.gso with (x:=Vint Int.one) (m:=(Maps.PTree.set _t'8 (Vint Int.one) le5)) in Hneq3; rewrite Hneq3.
+    apply Maps.PTree.gso with (x:=Vint Int.one) (m:=le5) in Hneq1; rewrite Hneq1.
+    rewrite p1; reflexivity.
+    reflexivity.
+    reflexivity.
+
+    (**r we need to show : Vint (Int.add vi10 vi3)) = v && m = m5 *)
+    simpl.
+    Check Maps.PTree.gso.
+    
+    simpl.
+
+
+    
+  admit.
+ 
   (* TODO .... *)
 
 
-  {
-    intros. (** l' is map_opt _ l' *)
-    apply match_temp_env_ex with (l':= [(_addr0, Clightdefs.tulong); (_start, Clightdefs.tulong)]) in H.
-    destruct H.
-    exists x2. split; auto.
-    apply length_map_opt in H.
-    rewrite <- H. reflexivity.
-    unfold INV, incl; simpl.
-    intuition subst;discriminate.
-  }
-  intros.
-
-
-
-  [
-          reflexivity
-          | reflexivity
-          | reflexivity
-          | typeclasses eauto
-          | idtac
-          | reflexivity
-          | reflexivity
-          | reflexivity
-          | reflexivity
-          | prove_incl
-          | prove_in_inv
-          | prove_in_inv
-          | idtac
-         ].
-  
-      [ change_app_for_statement ;
-        let b := match T with
-                 | Ecast _ _ => constr:(true)
-                 | _         => constr:(false)
-                 end in
-        eapply correct_statement_call with (has_cast := b);
-        [
-          reflexivity
-          | reflexivity
-          | reflexivity
-          | typeclasses eauto
-          | idtac
-          | reflexivity
-          | reflexivity
-          | reflexivity
-          | reflexivity
-          | prove_incl
-          | prove_in_inv
-          | prove_in_inv
-          | idtac
-         ]
-      |]
-  correct_forward.
-  unfold getMemRegion_block_ptr. Print correct_getMemRegion_block_ptr.correct_function3_getMemRegion_block_ptr.
-  unfold bindM.
-  unfold runM, returnM.
-  
-  match goal with
-    | |- @correct_body _ _ 
-  unfold getMemRegion_start_addr.
-  admit.
-  (* TODO *)
   repeat intro.
   repeat eexists.
   eapply Smallstep.star_step;eauto.
@@ -619,3 +617,5 @@ Admitted.
 
 
 End Check_mem_aux.
+
+Close Scope Z_scope.
