src/DxState.v
@@ -117,21 +117,33 @@ Definition upd_mem (m: Mem.mem) (st: state): state := {| (**r never be used I gu
 |}.
 
 Definition load_mem (chunk: memory_chunk) (ptr: valu32_t) (st: state) :=
-  match Mem.loadv chunk (bpf_m st) ptr with
-  | Some res => res
-  | None => val64_zero
+  match ptr with
+  | Vptr b ofs =>
+    match Mem.load chunk (bpf_m st) b (Ptrofs.unsigned ofs) with
+    | Some res => res
+    | None => val64_zero
+    end
+  | _ => val64_zero
   end.
 
 Definition store_mem_imm (chunk: memory_chunk) (ptr: valu32_t) (v: vals32_t) (st: state): state :=
-  match Mem.storev chunk (bpf_m st) ptr v with
-  | Some m => upd_mem m st
-  | None => upd_mem init_mem st
+  match ptr with
+  | Vptr b ofs =>
+    match Mem.store chunk (bpf_m st) b (Ptrofs.unsigned ofs) v with
+    | Some m => upd_mem m st
+    | None => upd_flag BPF_ILLEGAL_MEM st
+    end
+  | _ => upd_flag BPF_ILLEGAL_MEM st
   end.
 
 Definition store_mem_reg (chunk: memory_chunk) (ptr: valu32_t) (v: val64_t) (st: state): state :=
-  match Mem.storev chunk (bpf_m st) ptr v with
-  | Some m => upd_mem m st
-  | None => upd_mem init_mem st
+  match ptr with
+  | Vptr b ofs =>
+    match Mem.store chunk (bpf_m st) b (Ptrofs.unsigned ofs) v with
+    | Some m => upd_mem m st
+    | None => upd_flag BPF_ILLEGAL_MEM st
+    end
+  | _ => upd_flag BPF_ILLEGAL_MEM st
   end.
 
 (******************** Dx Related *******************)
